tweaks to Imp to make it easy to configure with NBE

examples/tactics/Imp.fst
@@ -17,8 +17,8 @@ type inst =
     | Sub : reg -> reg -> reg -> inst
     | Mul : reg -> reg -> reg -> inst
     | Const : rval -> reg -> inst
-    //| If0 : reg -> prog -> prog -> inst
-    //| Seq : prog -> inst
+    | If0 : reg -> prog -> prog -> inst
+    | Seq : prog -> inst
 and prog = list inst
 
 module L = FStar.List.Tot
@@ -28,12 +28,13 @@ let rec size : inst -> pos = function
   | Sub _ _ _
   | Mul _ _ _
   | Const _ _  -> 1
-  //| If0 _ i j -> 1 + size_l i + size_l j
-  //| Seq i -> 1 + size_l i
+  | If0 _ i j -> 1 + size_l i + size_l j
+  | Seq i -> 1 + size_l i
 
 and size_l : prog -> pos = function
   | [] -> 1
   | hd::tl -> size hd + size_l tl
+  
 val override : reg -> rval -> regmap -> regmap
 let override r v rm =
     fun r' ->
@@ -48,20 +49,36 @@ let rec eval' (i:inst) (rm:regmap)
       | Sub r1 r2 r3 -> override r3 (rm r1 - rm r2) rm
       | Mul r1 r2 r3 -> override r3 (rm r1 * rm r2) rm
       | Const v r    -> override r v rm
-      //| Seq []       -> rm
-//      | Seq (p::ps)   -> eval' (Seq ps) (eval' p rm)
-//      | If0 r p0 p1  ->
-//          if rm r = 0 
-//          then eval' (Seq p0) rm
-//          else eval' (Seq p1) rm
+      | Seq []       -> rm
+      | Seq (p::ps)   -> eval' (Seq ps) (eval' p rm)
+      | If0 r p0 p1  ->
+          if rm r = 0 
+          then eval' (Seq p0) rm
+          else eval' (Seq p1) rm
 
 (* Run in all zeros and get the 0th reg *)
 val eval : prog -> rval
-//let eval p = let rm = eval' (Seq p) (fun _ -> 0) in rm (R 0)
-let eval p = let rm = List.Tot.fold_left (fun r i -> eval' i r) (fun _ -> 0) p in rm (R 0)
-
+let eval p = let rm = eval' (Seq p) (fun _ -> 0) in rm (R 0)
 let equiv p1 p2 = eval p1 == eval p2
 
+irreducible
+let unfold_defs = ()
+
+unfold
+let normal #a (e:a) =
+  FStar.Pervasives.norm 
+           [zeta;
+            iota;
+            delta_only [`%eval; `%eval'; `%override]; 
+            delta_attr unfold_defs; 
+            primops// ;
+            // nbe
+  ] e
+
+unfold
+let equiv_norm p1 p2 = normal (eval p1) == normal (eval p2)
+
+[@unfold_defs]
 let mk42 : prog = [
     Const 1 (R 0);
     Add (R 0) (R 0) (R 1);
@@ -76,24 +93,28 @@ let mk42 : prog = [
 
 let _ = assert_norm (eval mk42 == 42)
 
+[@unfold_defs]
 let add1 x y : prog = [
     Const x (R 0);
     Const y (R 1);
     Add (R 0) (R 1) (R 0);
 ]
-    
+
+[@unfold_defs]
 let add2 x y : prog = [
     Const y (R 1);
     Const x (R 0);
     Add (R 0) (R 1) (R 0);
 ]
     
+[@unfold_defs]
 let add3 x y : prog = [
     Const x (R 0);
     Const y (R 1);
     Add (R 1) (R 0) (R 0);
 ]
     
+[@unfold_defs]
 let add4 x y : prog = [
     Const y (R 1);
     Const x (R 0);
@@ -102,25 +123,26 @@ let add4 x y : prog = [
 
 (* All of these identies are quite easy by normalization. Once we fix
  * #1482, they will not even require SMT. *)
-let _ = assert_norm (forall x y. equiv (add1 x y) (add2 x y))
-let _ = assert_norm (forall x y. equiv (add1 x y) (add3 x y))
-let _ = assert_norm (forall x y. equiv (add1 x y) (add4 x y))
-let _ = assert_norm (forall x y. equiv (add2 x y) (add3 x y))
-let _ = assert_norm (forall x y. equiv (add2 x y) (add4 x y))
-let _ = assert_norm (forall x y. equiv (add3 x y) (add4 x y))
+#set-options "--max_fuel 0"
+let _ = assert (forall x y. equiv_norm (add1 x y) (add2 x y))
+let _ = assert (forall x y. equiv_norm (add1 x y) (add3 x y))
+let _ = assert (forall x y. equiv_norm (add1 x y) (add4 x y))
+let _ = assert (forall x y. equiv_norm (add2 x y) (add3 x y))
+let _ = assert (forall x y. equiv_norm (add2 x y) (add4 x y))
+let _ = assert (forall x y. equiv_norm (add3 x y) (add4 x y))
+
 
 (* Without normalizing, they require fuel, or else fail *)
-#push-options "--max_fuel 0"
 [@Pervasives.fail] let _ = assert (forall x y. equiv (add1 x y) (add2 x y))
 [@Pervasives.fail] let _ = assert (forall x y. equiv (add1 x y) (add3 x y))
 [@Pervasives.fail] let _ = assert (forall x y. equiv (add1 x y) (add4 x y))
 [@Pervasives.fail] let _ = assert (forall x y. equiv (add2 x y) (add3 x y))
 [@Pervasives.fail] let _ = assert (forall x y. equiv (add2 x y) (add4 x y))
 [@Pervasives.fail] let _ = assert (forall x y. equiv (add3 x y) (add4 x y))
-#pop-options
 
 (* poly5 x = x^5 + x^4 + x^3 + x^2 + x^1 + 1 *)
 
+[@unfold_defs]
 let poly5 x : prog = [
     Const 1 (R 0);
     Const x (R 1);
@@ -135,18 +157,19 @@ let poly5 x : prog = [
     Add (R 0) (R 5) (R 0);
 ]
 
-let _ = assert_norm (eval (poly5 1) == 6)
-let _ = assert_norm (eval (poly5 2) == 63)
-let _ = assert_norm (eval (poly5 3) == 3*3*3*3*3 + 3*3*3*3 + 3*3*3 + 3*3 + 3 + 1)
+let _ = assert (normal (eval (poly5 1)) == 6)
+let _ = assert (normal (eval (poly5 2)) == 63)
+let _ = assert (normal (eval (poly5 3)) == 3*3*3*3*3 + 3*3*3*3 + 3*3*3 + 3*3 + 3 + 1)
 
 (* Bunch of fuel to even prove ground facts *)
-//#push-options "--max_fuel 12"
-//let _ = assert (eval (poly5 1) == 6)
-//let _ = assert (eval (poly5 2) == 63)
-//let _ = assert (eval (poly5 3) == 3*3*3*3*3 + 3*3*3*3 + 3*3*3 + 3*3 + 3 + 1)
-//#pop-options
+#reset-options "--initial_fuel 100 --max_fuel 100"
+let _ = assert (eval (poly5 1) == 6)
+let _ = assert (eval (poly5 2) == 63)
+let _ = assert (eval (poly5 3) == 3*3*3*3*3 + 3*3*3*3 + 3*3*3 + 3*3 + 3 + 1)
+#reset-options "--max_fuel 0"
 
 (* A different way of computing it *)
+[@unfold_defs]
 let poly5' x : prog = [
     Const 1 (R 0);
     Const x (R 1);
@@ -164,32 +187,32 @@ let poly5' x : prog = [
 ]
 
 (* Seems to do the same *)
-let _ = assert_norm (eval (poly5' 1) == 6)
-let _ = assert_norm (eval (poly5' 2) == 63)
-let _ = assert_norm (eval (poly5' 3) == 3*3*3*3*3 + 3*3*3*3 + 3*3*3 + 3*3 + 3 + 1)
+let _ = assert (normal (eval (poly5' 1)) == 6)
+let _ = assert (normal (eval (poly5' 2)) == 63)
+let _ = assert (normal (eval (poly5' 3)) == 3*3*3*3*3 + 3*3*3*3 + 3*3*3 + 3*3 + 3 + 1)
 
 (* Same *)
-#push-options "--max_fuel 20"
-//let _ = assert (eval (poly5' 1) == 6)
-//let _ = assert (eval (poly5' 2) == 63)
-//let _ = assert (eval (poly5' 3) == 3*3*3*3*3 + 3*3*3*3 + 3*3*3 + 3*3 + 3 + 1)
-//let _ = assert (forall x. poly5 x `equiv` poly5' x)
-#pop-options
-
-//[@Pervasives.fail]
-//let _ = assert (forall x. poly5 x `equiv` poly5' x)
-//
-//#set-options "--z3rlimit 10"
-//let _ = assert_norm (forall x. (poly5 (eval (poly5 x)) `equiv` poly5' (eval (poly5' x))))
-
-#set-options "--max_fuel 0"
-// --tactic_trace"
+#reset-options "--initial_fuel 100 --max_fuel 100"
+let _ = assert (eval (poly5' 1) == 6)
+let _ = assert (eval (poly5' 2) == 63)
+let _ = assert (eval (poly5' 3) == 3*3*3*3*3 + 3*3*3*3 + 3*3*3 + 3*3 + 3 + 1)
 let _ = assert (forall x. poly5 x `equiv` poly5' x)
-          by (fun () -> let _ = forall_intros () in
-		     compute ();
-		     dump "after norm";
-		     canon_semiring int_cr;
-		     dump "final")
+#reset-options "--max_fuel 0"
+
+// [@Pervasives.fail]
+// let _ = assert (forall x. poly5 x `equiv` poly5' x)
+
+// #set-options "--z3rlimit 10"
+// let _ = assert_norm (forall x. (poly5 (eval (poly5 x)) `equiv` poly5' (eval (poly5' x))))
+
+// #set-options "--max_fuel 0"
+// // --tactic_trace"
+// let _ = assert (forall x. poly5 x `equiv` poly5' x)
+//           by (fun () -> let _ = forall_intros () in
+// 		     compute ();
+// 		     dump "after norm";
+// 		     canon_semiring int_cr;
+// 		     dump "final")
 
 // Takes long.. try again later
 //let _ = assert (forall x. (poly5 (eval (poly5 x)) `equiv` poly5' (eval (poly5' x))))
